FOL/NV/Margaris/Deduct.lean
@@ -1,4 +1,4 @@
-import FOL.Sub.One.Rec.SubOneRecAdmits
+import FOL.NV.Sub.One.Rec.SubOneRecAdmits
 import FOL.Tactics
 
 
