FOL/NV/Sub/One/Rec/SubOneRecReplaceFree.lean
@@ -1,5 +1,5 @@
+import FOL.NV.Binders
 import FOL.List
-import FOL.Binders
 import FOL.Tactics
 
 
